formalization/thesis/Isotope/LambdaCase/Subtyping.lean
@@ -1,0 +1,4 @@
+import Isotope.LambdaCase.Subtyping.Typing
+import Isotope.LambdaCase.Subtyping.TypingSubst
+import Isotope.LambdaCase.Subtyping.Equiv
+import Isotope.LambdaCase.Subtyping.Semantics.Categorical
